HeapMemory.thy
@@ -21,8 +21,13 @@ inductive evalh :: "heap_state \<Rightarrow> heap_state \<Rightarrow> bool" (inf
 | evh_apply [simp]: "cd ! pc = BApply \<Longrightarrow> hlookup h v2 = HLam env pc' \<Longrightarrow>
     HS h (v1 # v2 # vs) envs (Suc pc # pcs) cd \<leadsto>\<^sub>h
       HS h vs ((v1 # env) # envs) (pc' # pc # pcs) cd"
-| evh_return [simp]: "cd ! pc = BReturn \<Longrightarrow> 
+| evh_return [simp]: "cd ! pc = BReturn_Old \<Longrightarrow> 
     HS h vs envs (Suc pc # pcs) cd \<leadsto>\<^sub>h HS h vs envs pcs cd"
+| evh_returnb [simp]: "cd ! pc = BReturn \<Longrightarrow> 
+    HS h vs (env # envs) (Suc pc # pcs) cd \<leadsto>\<^sub>h HS h vs envs pcs cd"
+| evh_jump [simp]: "cd ! pc = BJump \<Longrightarrow> hlookup h v2 = HLam env' pc' \<Longrightarrow>
+    HS h (v1 # v2 # vs) (env # envs) (Suc pc # pcs) cd \<leadsto>\<^sub>h 
+      HS h vs ((v1 # env') # envs) (pc' # pcs) cd"
 
 theorem determinismh: "\<Sigma> \<leadsto>\<^sub>h \<Sigma>' \<Longrightarrow> \<Sigma> \<leadsto>\<^sub>h \<Sigma>'' \<Longrightarrow> \<Sigma>' = \<Sigma>''"
 proof (induction \<Sigma> \<Sigma>' rule: evalh.induct)
@@ -50,6 +55,15 @@ next
   case (evh_return cd pc h vs envs pcs)
   from evh_return(2, 1) show ?case 
     by (induction "HS h vs envs (Suc pc # pcs) cd" \<Sigma>'' rule: evalh.induct) simp_all 
+next
+  case (evh_returnb cd pc h vs env envs pcs)
+  from evh_returnb(2, 1) show ?case 
+    by (induction "HS h vs (env # envs) (Suc pc # pcs) cd" \<Sigma>'' rule: evalh.induct) simp_all 
+next
+  case (evh_jump cd pc h v2 env' pc' v1 vs env envs pcs)
+  from evh_jump(3, 1, 2) show ?case 
+    by (induction "HS h (v1 # v2 # vs) (env # envs) (Suc pc # pcs) cd" \<Sigma>'' rule: evalh.induct) 
+       simp_all 
 qed
 
 lemma [simp]: "\<Sigma> \<leadsto>\<^sub>h \<Sigma>' \<Longrightarrow> code \<Sigma> = code \<Sigma>'"
